dijkstra/SpaceDijkGraph3.v
@@ -6,12 +6,15 @@ Local Open Scope logic.
 
 Section SpaceDijkGraph.
 
+  Context {V_EqDec : EquivDec.EqDec V eq}. 
+  Context {E_EqDec : EquivDec.EqDec E eq}. 
+
   Lemma elabel_Znth_graph_to_mat:
-    forall (g: @DijkGG size inf) src dst,
+    forall (g: @DijkGG size inf _ _) src dst,
       vvalid g src ->
       vvalid g dst ->
       elabel g (src, dst) =
-      Znth dst (Znth src (@graph_to_mat size g id)).
+      Znth dst (Znth src (@graph_to_mat size _ _ g id)).
   Proof.
     intros.
     rewrite (vvalid_meaning g) in H, H0.
@@ -20,7 +23,7 @@ Section SpaceDijkGraph.
     lia.
   Qed.
 
-  Definition DijkGraph sh cs g g_ptr size (addresses: list val) : mpred := @SpaceAdjMatGraph size cs sh id g g_ptr.
+  Definition DijkGraph sh cs g g_ptr size (addresses: list val) : mpred := @SpaceAdjMatGraph size cs _ _ sh id g g_ptr.
   (* "addresses" is accepted but not used *)
   (* the user should just give a nil list *)
 
